src/ConcreteEvidence.v
@@ -24,7 +24,8 @@ Inductive EvidenceC: Set :=
 | nnc: N_ID -> BS -> EvidenceC
 | ggc: Plc -> ASP_PARAMS -> BS -> EvidenceC -> EvidenceC
 | hhc: Plc -> ASP_PARAMS -> BS -> Evidence -> EvidenceC
-| eec: Plc -> ASP_PARAMS -> BS -> EvidenceC -> EvidenceC
+| eec: Plc -> ASP_PARAMS -> BS -> Evidence -> EvidenceC
+| kkc: Plc -> ASP_PARAMS -> Evidence -> EvidenceC
 | ssc: EvidenceC -> EvidenceC -> EvidenceC.
 
 (** The Evidence Type associated with a Typed Concrete Evidence value *)
@@ -33,7 +34,8 @@ Fixpoint et_fun (ec:EvidenceC) : Evidence :=
   | mtc => mt
   | ggc p params _ ec' => uu p EXTD params (et_fun ec')
   | hhc p params _ et => uu p COMP params et
-  | eec p params _ ec' => uu p ENCR params (et_fun ec')
+  | eec p params _ et => uu p ENCR params et (* (et_fun ec') *)
+  | kkc _ _ _ => mt
   | nnc ni _ => nn ni
   | ssc ec1 ec2 => ss (et_fun ec1) (et_fun ec2)
   end.
@@ -116,12 +118,19 @@ Proof.
   -
     invc H0.
     jkjke.
-    assert (e' = mtc).
+    assert (e' = mtc \/ (exists p ps et', e' = kkc p ps et')).
     {
       destruct e'; try solve_by_inversion.
+      eauto.
     }
+    door.
+    +
     subst.
     ff.
+    +
+      subst.
+      ff.
+      
   -
     invc H0.
     jkjke.
